IntrinsicProofs.v
@@ -1,0 +1,405 @@
+From mathcomp Require Import ssreflect ssrnat ssrbool.
+Set Bullet Behavior "Strict Subproofs".
+
+From MonadicEffect Require Import Trees.
+
+(** * Extrinsic and Intrinsic Proofs
+
+    There are two types of proofs: _extrinsic_ ones and _intrisic_
+    ones. An extrinsic proof is what most people familiar with in Coq:
+    you write down a function, and then prove some properties about
+    it. In a intrinsic proof, however, you write the properties in the
+    type of the function.
+
+    Let's just jump into an example to show what they look like. We
+    start with the more familiar extrinsic approach. *)
+
+Section ExtrinsicProof.
+
+  Variable A : Set.
+
+  (** We import state monads from coq-ext-lib. *)
+  From ExtLib Require Import Structures.Monads Data.Monads.StateMonad.
+  Import MonadNotation.
+  Local Open Scope monad_scope.
+
+  (** Consider the following [relabel] function. It labels all leaves
+      in a tree in with [nat]s in an increasing order. It maintains a
+      counter using the state monad. *)
+  Fixpoint relabel (t : Tree A) : state nat (Tree nat) :=
+    match t with
+    | Leaf x =>
+      n <- get ;;
+      put (n + 1) ;;
+      ret (Leaf n)
+    | Node l r =>
+      l' <- relabel l ;;
+      r' <- relabel r ;;
+      ret (Node l' r')
+    end.
+
+  (** Now we can write down a specification of this function and prove
+      it. *)
+  Theorem relabel_spec : forall t s,
+      let: (t', s') := runState (relabel t) s in
+      s' = s + size t' /\ flatten t' = seq s (size t').
+  Proof.
+    (** The proof starts by doing induction on the tree. The [Leaf]
+        case is trivial, and can be dischagred automatically. *)
+    elim => // => l IHt1 r IHt2 s.
+    (** In the [Node] case, we do some rewriting to expose the
+        computation on left and right children, so we can use our
+        induction hypotheses. *)
+    rewrite /relabel /= -/relabel.
+    (** Now we need a bit boilerplates to destruct the [let]s
+        generated from [bind]s, and pass the states through. *)
+    specialize (IHt1 s). 
+    destruct (runState (relabel l) s) as [t' s'].
+    specialize (IHt2 s').
+    destruct (runState (relabel r) s') as [t'' s''].
+    split => /=; intuition; subst.
+    - by rewrite addnA.
+    - by rewrite H0 H2 seq_split.
+  Qed.
+End ExtrinsicProof.
+  (** The proof is quite standard. There are a bit boilerplates with
+      [bind]s. Can we make use of the monadic structure to propagate
+      the proof?
+
+      The intrinsic approach offers one solution to that. Let's see
+      how we prove the same thing in that style. *)
+
+(* begin hide *)
+Reset ExtrinsicProof.
+(* end hide *)
+Section IntrinsicProof.
+
+  Variable A : Set.
+
+  (** Here we use something called [Dijkstra] monads we have already
+      defined. We will show to define it later. *)
+  From MonadicEffect Require Import Dijkstra.
+
+  (** This time, we enhance the type of the [relabel] function, by
+      putting a pre- and post-condition in its type. By using the
+      [Program] feature provided by Coq, we can define this function
+      with the function body exactly the same as before. One
+      difference is that now Coq will ask us to prove that the result
+      of this function indeed satisfies the post-condition. *)
+  Program Fixpoint relabel {A : Set} (t : Tree A) :
+    ST nat return (Tree nat)
+         requires [fun _ => True]
+         ensures  [fun s t s' => s' = s + size t /\ flatten t = seq s (size t)] :=
+  match t with
+  | Leaf x =>
+    n <- get ;;
+    put (n + 1) ;;
+    ret (Leaf n)
+  | Node l r =>
+    l' <- relabel l ;;
+    r' <- relabel r ;;
+    ret (Node l' r')
+  end.
+  (** Coq will try to automatically prove some simple proof
+      obligations for us. For this function, the case when [t] is a
+      [Leaf] is trivial, so Coq has already proved it for us.
+      
+      We only need to consider the case when [t] is a [Node]. The
+      proof is quite similar to the last part of the extrinsic
+      proof. *)
+  Next Obligation.
+    repeat split => //.
+    intros; destruct H0; destruct H; subst.
+    apply x1. split => /=. 
+    - by rewrite addnA.
+    - by rewrite H2 H1 seq_split.
+  Defined.
+End IntrinsicProof.
+
+(* begin hide *)
+Reset IntrinsicProof.
+(* end hide *)
+(** * Intrinsic Proofs in Coq
+
+    Before we jump into the details how the above example is
+    implemented in Coq, let's check a little bit technical details in
+    Coq. *)
+Section IntrinsicProof.
+
+  Fail Definition sqr (x : nat) : { s : nat | s = x * x } :=
+    x * x.
+
+  Print sig.
+
+(** The signature of subset types:
+<<
+Inductive sig (A : Type) (P : A -> Prop) : Type :=
+    exist : forall x : A, P x -> {x : A | P x}
+
+For sig: Argument A is implicit
+For exist: Argument A is implicit
+For sig: Argument scopes are [type_scope type_scope]
+For exist: Argument scopes are [type_scope function_scope _ _] 
+>> *)
+
+  Definition sqr (x : nat) : { s : nat | s = x * x } :=
+    exist (fun s => s = x * x) (x * x) eq_refl.
+
+  Reset sqr.
+
+  Definition sqr (x : nat) : { s : nat | s = x * x }.
+    refine (exist _ (x * x) _).
+    reflexivity.
+  Defined.
+
+  Reset sqr.
+
+  (** Coq's [Program] feature allows us to program with subset types
+      without worrying about passing the proof objects. *)
+  Program Definition sqr (x : nat) : { s : nat | s = x * x } := x * x.
+
+End IntrinsicProof.
+
+(* begin hide *)
+Reset IntrinsicProof.
+(* end hide *)
+Require Import Program.
+
+(** * The Hoare State Monad
+
+    Most of this section is based on [Swierstra, W. (2009). A Hoare
+    Logic for the State Monad]. *)
+
+Section HoareStateMonads.
+
+  Variable S : Set.
+  
+  Definition Pre : Type := S -> Prop.
+  Definition Post (A : Set) : Type := S -> A -> S -> Prop.
+  
+  Program Definition HoareState (pre : Pre) (A : Set) (post : Post A) : Set :=
+    forall s: { s : S | pre s }, { (a, s') : A * S | post s a s' }.
+
+  Definition top : Pre := fun _ => True.
+
+  (** Recall the type of [ret] for an ordinary state monad is
+
+      <<
+      A -> state S A
+      >> *)
+  Program Definition ret (A : Set) :
+    forall a, HoareState top A (fun s a' s' => s = s' /\ a = a') :=
+    fun a s => (a, s).
+
+  (** Recall the type of [bind] for an ordinary state monad is
+
+      << state S A -> (A -> state S B) -> state S B >>
+      
+      Note the use of dependent type in our second parameter
+      below. The reason is that we would like to refer to [a] in the
+      pre- and post-conditions of the second parametr!  *)
+  Program Definition bind : forall A B P1 P2 Q1 Q2,
+      HoareState P1 A Q1 ->
+      (forall (a : A), HoareState (P2 a) B (Q2 a)) ->
+      HoareState (fun s1 => P1 s1 /\ forall a s2, Q1 s1 a s2 -> P2 a s2)
+                  B
+                  (fun s1 a' s3 => exists a, exists s2, Q1 s1 a s2 /\ Q2 a s2 a' s3) :=
+    fun A B P1 P2 Q1 Q2 m1 m2 s1 =>
+      let: (a, s2) := m1 s1 in m2 a s2.
+  Next Obligation.
+    (** The first obligation is proving that [a] and [s2] satisfies
+        the precontion of [m2]. *)
+    elim: m1 Heq_anonymous => t /= H0 Heq_anonymous.
+    subst. by apply p0.
+  Defined.
+  Next Obligation.
+    (** The second obligation is proving that [m2 a s2] satisfies the
+        post condition of [bind]. *)
+    elim (m2 a) => /=. elim => a' s3 H.
+    exists a. exists s2. split; auto.
+    elim: m1 Heq_anonymous => t /= H0 Heq_anonymous.
+    subst. by apply H0.
+  Defined.
+
+  (** [get] and [put] are straightforward. *)
+  Program Definition get : HoareState top S (fun s a s' => s = s' /\ a = s) :=
+    fun s => (s, s).
+  Program Definition put (x : S) : HoareState top unit (fun _ _ s' => x = s') :=
+    fun _ => (tt, x).
+End HoareStateMonads.
+
+(* begin hide *)
+Arguments ret {S} {A}.
+Arguments bind {S} {A} {B} {P1} {P2} {Q1} {Q2}.
+Arguments get {S}.
+Arguments put {S}.
+(* end hide *)
+(** We define some notations to use this monad more easily. *)
+Notation "c >>= f" := (bind c f) (at level 50, left associativity).
+Notation "f =<< c" := (bind c f) (at level 51, right associativity).
+Notation "x <- c1 ;; c2" := (bind c1 (fun x => c2)) (at level 100, c1 at next level, right associativity).
+Notation "e1 ;; e2" := (_ <- e1 ;; e2) (at level 100, right associativity).
+
+(** Now we can do an intrinsic proof to show that our [relabel]
+    function is correct with respect to its specification again. *)
+Program Fixpoint relabel {A : Set} (t : Tree A) :
+  HoareState nat
+             (@top nat)
+             (Tree nat) 
+             (fun i t f => f = i + size t /\ flatten t = seq i (size t)) :=
+  match t with
+  | Leaf x =>
+    n <- get ;;
+    put (n + 1) ;;
+    ret (Leaf n)
+  | Node l r =>
+    l' <- relabel l ;;
+    r' <- relabel r ;;
+    ret (Node l' r')
+  end.
+Next Obligation.
+  case (relabel A l >>= _) => /=.
+  case=> a s' [a1] [s1] [[H0 H1] H2].
+  case: H2 => a2 [s2] [[H3 H4] [H5 H6]].  
+  subst. split => /=.
+  - by rewrite addnA.
+  - by rewrite H1 H4 seq_split.
+Defined.
+
+(** * Dijkstra Monads
+
+    The Hoare state monad we have implemented have a few
+    disadvantages, according to [Swamy, N., Weinberger, J.,
+    Schlesinger, C., Chen, J., & Livshits, B. (2013). Verifying
+    higher-order programs with the dijkstra monad]:
+
+    - There are some existential quantifiers in it. Reasoning with
+      these quantifiers, particularly using automated SMT solvers, can
+      be problematic.
+
+    - It requires the post-condition to be a two-state relation,
+      though sometimes it is not necessary to compare the two states
+      in the specification.
+
+    Therefore, they propose another monad called "Dijkstra monad" to
+    resolve the above issues (name after Edsger W. Dijkstra, for his
+    discoveries in his paper [Dijkstra, E. W. (1975). Guarded
+    Commands, Nondeterminacy and Formal Derivation of Programs].
+
+    A Dijkstra monad is parameterized over a weakest precondition
+    transformer. It can be seen as a Hoare state monad: *)
+
+Definition DST S A wp :=
+  forall p, HoareState S (fun h => wp p h) A (fun h x h' => p x h').
+
+(** But let's define it properly. *)
+Reset HoareStateMonads.
+
+Section DijkstraMonads.
+
+  Variables S : Set.
+
+  (** The weakest precondition transformer. As its name suggested, it
+      takes a post-condition and transform it into the weakest
+      precondition. *)
+  Definition WP {A} : Type := (A -> S -> Prop) -> S -> Prop.
+
+  Program Definition DST A (wp : WP) :=
+    forall p, { s : S | wp p s } -> { (a, s') : A * S | p a s' }.
+
+  Program Definition ret { A } (a : A) :
+    DST A (fun p => p a) :=
+    fun _ s => (a, s).
+
+  Program Definition bind : forall A wp1 B wp2,
+      DST A wp1 -> (forall a : A, DST B (wp2 a)) ->
+      DST B (fun p => wp1 (fun a => wp2 a p)) :=
+    fun A wp1 B wp2 c1 c2 p s1 =>
+      (** The function body should be
+
+          <<
+          let: (a, s2) := c1 (fun a => wp2 a p) s1 in c2 a p s2.
+          >>
+          But we can also just write this: *)
+  let: (a, s2) := c1 _ s1 in c2 a _ s2.
+  Next Obligation.
+    elim: c1 Heq_anonymous => a' H' /= Heq_anonymous.
+    subst; done.
+  Defined.
+
+  Program Definition get : DST S (fun p s => p s s) :=
+    fun _ s => (s, s).
+
+  Program Definition put : forall s, DST unit (fun p _ => p tt s) :=
+    fun s _ _ => (tt, s).
+  
+End DijkstraMonads.
+
+Arguments ret {S} {A}.
+Arguments bind {S} {A} {wp1} {B} {wp2}.
+Arguments get {S}.
+Arguments put {S}.
+
+Notation "c >>= f" := (bind c f) (at level 50, left associativity).
+Notation "f =<< c" := (bind c f) (at level 51, right associativity).
+Notation "x <- c1 ;; c2" := (bind c1 (fun x => c2)) (at level 100, c1 at next level, right associativity).
+Notation "e1 ;; e2" := (_ <- e1 ;; e2) (at level 100, right associativity).
+
+(** Let's see how it works with our [relabel] function: *)
+Program Fixpoint relabel {A : Set} (t : Tree A) :
+  DST nat (Tree nat) (fun p s =>
+                    forall t s', s' = s + size t /\ flatten t = seq s (size t) ->
+                    p t s' ) :=
+  match t with
+  | Leaf x =>
+    n <- get ;;
+    put (n + 1) ;;
+    ret (Leaf n)
+  | Node l r =>
+    l' <- relabel l ;;
+    r' <- relabel r ;;
+    ret (Node l' r')
+  end.
+Next Obligation.
+  (** We show the function satisfies the post-condition. To do that,
+      we show that it satisfies the weakest precondition. *)
+  apply H3. split => /=.
+  - by rewrite addnA.
+  - by rewrite H2 H1 seq_split.
+Defined.
+
+(** Writing with weakest precondition transformer can sometimes be
+    hard. We can define some notations to make it more intuitive. *)
+Reset relabel.
+
+Notation "'ST' s 'return' a 'requires' [ P ] 'ensures' [ Q ]" :=
+  (DST s a (fun p s1 => P s1 /\ (forall c s2, Q s1 c s2 -> p c s2)))
+    (at level 99, P at next level, Q at next level).
+
+Notation "'ST' s 'return' a 'ensures' [ Q ]" :=
+  (DST s a (fun p s1 => forall c s2, Q s1 c s2 -> p c s2))
+    (at level 99, Q at next level).
+
+Check (ST nat return (Tree nat) requires [fun _ => True] ensures [fun _ _ _ => True]).
+
+(** Now the specification for [relabel] looks quite similar to that in
+    the form of a Hoare state monad, but notice that the proof is
+    simpler than that for a Hoare state monad. *)
+Program Fixpoint relabel {A : Set} (t : Tree A) :
+  ST nat return (Tree nat)
+       ensures  [fun i t f => f = i + size t /\ flatten t = seq i (size t)] :=
+match t with
+| Leaf x =>
+  n <- get ;;
+  put (n + 1) ;;
+  ret (Leaf n)
+| Node l r =>
+  l' <- relabel l ;;
+  r' <- relabel r ;;
+  ret (Node l' r')
+end.
+Next Obligation.
+  apply H3. split => /=. 
+  - by rewrite addnA.
+  - by rewrite H2 H1 seq_split.
+Defined.
